Tentative first fix for offsets of ld/std.
The offsets immediates used in the ld and std instructions must be a
multiple of the word size. This commit changes the two functions which
are used when generating load/stores in Asmgen, accessind and
transl_memory_access.

For accessind one only needs an additional check that the offset is a
multiple of the word size for the case that the high part of the offset
is zero, since otherwise the immediate is loaded into a register anyway.

The transl_memory_access function needs some slightly more complex
adoption. For all variants that do not construct the address in a
register before hand we must check that the offsets are multiples of the
word size and additionally if a symbol is used that the alignment of the
symbol is also a multiple of the word size. Therefore a new parameter is
introduced that allows checking the alignment.

In order to reduce the code duplication for the proofs these two
functions get an additional parameter in order to indicate wether the
offset needs to be a multiple of the word size or not.
Bug 30983

powerpc/Asmgen.v
@@ -190,36 +190,38 @@ Definition rolm64 (r1 r2: ireg) (amount: int) (mask: int64) (k: code) :=
 
 (** Accessing slots in the stack frame.  *)
 
+(* For 64 bit load and store the offset needs to be a multiple of word size *)
 Definition accessind {A: Type}
        (instr1: A -> constant -> ireg -> instruction)
        (instr2: A -> ireg -> ireg -> instruction)
+       (unaligned : bool)
        (base: ireg) (ofs: ptrofs) (r: A) (k: code) :=
   let ofs := Ptrofs.to_int ofs in
-  if Int.eq (high_s ofs) Int.zero
+  if Int.eq (high_s ofs) Int.zero && (unaligned || (Int.eq (Int.mods ofs (Int.repr 4)) Int.zero))
   then instr1 r (Cint ofs) base :: k
   else loadimm GPR0 ofs (instr2 r base GPR0 :: k).
 
 Definition loadind (base: ireg) (ofs: ptrofs) (ty: typ) (dst: mreg) (k: code) :=
   match ty, preg_of dst with
-  | Tint, IR r => OK(accessind Plwz Plwzx base ofs r k)
-  | Tany32, IR r => OK(accessind Plwz_a Plwzx_a base ofs r k)
-  | Tsingle, FR r => OK(accessind Plfs Plfsx base ofs r k)
-  | Tlong, IR r => OK(accessind Pld Pldx base ofs r k)
-  | Tfloat, FR r => OK(accessind Plfd Plfdx base ofs r k)
-  | Tany64, IR r => OK(accessind Pld_a Pldx_a base ofs r k)
-  | Tany64, FR r => OK(accessind Plfd_a Plfdx_a base ofs r k)
+  | Tint, IR r => OK(accessind Plwz Plwzx true base ofs r k)
+  | Tany32, IR r => OK(accessind Plwz_a Plwzx_a true base ofs r k)
+  | Tsingle, FR r => OK(accessind Plfs Plfsx true base ofs r k)
+  | Tlong, IR r => OK(accessind Pld Pldx false base ofs r k)
+  | Tfloat, FR r => OK(accessind Plfd Plfdx  true base ofs r k)
+  | Tany64, IR r => OK(accessind Pld_a Pldx_a false base ofs r k)
+  | Tany64, FR r => OK(accessind Plfd_a Plfdx_a true base ofs r k)
   | _, _ => Error (msg "Asmgen.loadind")
   end.
 
 Definition storeind (src: mreg) (base: ireg) (ofs: ptrofs) (ty: typ) (k: code) :=
   match ty, preg_of src with
-  | Tint, IR r => OK(accessind Pstw Pstwx base ofs r k)
-  | Tany32, IR r => OK(accessind Pstw_a Pstwx_a base ofs r k)
-  | Tsingle, FR r => OK(accessind Pstfs Pstfsx base ofs r k)
-  | Tlong, IR r => OK(accessind Pstd Pstdx base ofs r k)
-  | Tfloat, FR r => OK(accessind Pstfd Pstfdx base ofs r k)
-  | Tany64, IR r => OK(accessind Pstd_a Pstdx_a base ofs r k)
-  | Tany64, FR r => OK(accessind Pstfd_a Pstfdx_a base ofs r k)
+  | Tint, IR r => OK(accessind Pstw Pstwx true base ofs r k)
+  | Tany32, IR r => OK(accessind Pstw_a Pstwx_a true base ofs r k)
+  | Tsingle, FR r => OK(accessind Pstfs Pstfsx true base ofs r k)
+  | Tlong, IR r => OK(accessind Pstd Pstdx false base ofs r k)
+  | Tfloat, FR r => OK(accessind Pstfd Pstfdx true base ofs r k)
+  | Tany64, IR r => OK(accessind Pstd_a Pstdx_a false base ofs r k)
+  | Tany64, FR r => OK(accessind Pstfd_a Pstfdx_a true base ofs r k)
   | _, _ => Error (msg "Asmgen.storeind")
   end.
 
@@ -724,32 +726,48 @@ Definition transl_op
 Definition int_temp_for (r: mreg) :=
   if mreg_eq r R12 then GPR11 else GPR12.
 
+Definition symbol_ofs_word_aligned symb ofs :=
+  let ofs := Ptrofs.to_int ofs in
+  symbol_is_aligned symb 4 && (Int.eq (Int.mods ofs (Int.repr 4)) Int.zero).
+
 Definition transl_memory_access
      (mk1: constant -> ireg -> instruction)
      (mk2: ireg -> ireg -> instruction)
+     (unaligned : bool)
      (addr: addressing) (args: list mreg)
      (temp: ireg) (k: code) :=
   match addr, args with
   | Aindexed ofs, a1 :: nil =>
       do r1 <- ireg_of a1;
-      OK (if Int.eq (high_s ofs) Int.zero then
-           mk1 (Cint ofs) r1 :: k
-         else
-           Paddis temp r1 (Cint (high_s ofs)) ::
-           mk1 (Cint (low_s ofs)) temp :: k)
+      OK (if unaligned || Int.eq (Int.mods ofs (Int.repr 4)) Int.zero then
+            if Int.eq (high_s ofs) Int.zero then
+               mk1 (Cint ofs) r1 :: k
+             else
+               Paddis temp r1 (Cint (high_s ofs)) ::
+               mk1 (Cint (low_s ofs)) temp :: k
+          else
+            (loadimm GPR0 ofs (mk2 r1 GPR0 :: k)))
   | Aindexed2, a1 :: a2 :: nil =>
       do r1 <- ireg_of a1; do r2 <- ireg_of a2;
       OK (mk2 r1 r2 :: k)
   | Aglobal symb ofs, nil =>
-      OK (if symbol_is_small_data symb ofs then
-           mk1 (Csymbol_sda symb ofs) GPR0 :: k
+       OK (if symbol_is_small_data symb ofs then
+             if unaligned || symbol_ofs_word_aligned symb ofs then
+               mk1 (Csymbol_sda symb ofs) GPR0 :: k
+             else
+               Paddi temp GPR0 (Csymbol_sda symb ofs) ::
+               mk1 (Cint Int.zero) temp :: k
          else if symbol_is_rel_data symb ofs then
            Paddis temp GPR0 (Csymbol_rel_high symb ofs) ::
            Paddi temp temp (Csymbol_rel_low symb ofs) ::
            mk1 (Cint Int.zero) temp :: k
+         else if  unaligned || symbol_ofs_word_aligned symb ofs then
+           Paddis temp GPR0 (Csymbol_high symb ofs) ::
+           mk1 (Csymbol_low symb ofs) temp :: k
          else
            Paddis temp GPR0 (Csymbol_high symb ofs) ::
-           mk1 (Csymbol_low symb ofs) temp :: k)
+           Paddi temp temp (Csymbol_low symb ofs) ::
+           mk1 (Cint Int.zero) temp :: k)
   | Abased symb ofs, a1 :: nil =>
       do r1 <- ireg_of a1;
       OK (if symbol_is_small_data symb ofs then
@@ -760,16 +778,24 @@ Definition transl_memory_access
             Paddis temp GPR0 (Csymbol_rel_high symb ofs) ::
             Paddi temp temp (Csymbol_rel_low symb ofs) ::
             mk2 temp GPR0 :: k
-          else
+          else if  unaligned || symbol_ofs_word_aligned symb ofs then
             Paddis temp r1 (Csymbol_high symb ofs) ::
-            mk1 (Csymbol_low symb ofs) temp :: k)
+            mk1 (Csymbol_low symb ofs) temp :: k
+          else
+            Pmr GPR0 r1 ::
+            Paddis temp GPR0 (Csymbol_high symb ofs) ::
+            Paddi temp temp (Csymbol_low symb ofs) ::
+            mk2 temp GPR0 :: k)
   | Ainstack ofs, nil =>
       let ofs := Ptrofs.to_int ofs in
-      OK (if Int.eq (high_s ofs) Int.zero then
-           mk1 (Cint ofs) GPR1 :: k
-         else
-           Paddis temp GPR1 (Cint (high_s ofs)) ::
-           mk1 (Cint (low_s ofs)) temp :: k)
+      OK (if  unaligned || Int.eq (Int.mods ofs (Int.repr 4)) Int.zero then
+            if Int.eq (high_s ofs) Int.zero then
+              mk1 (Cint ofs) GPR1 :: k
+            else
+              Paddis temp GPR1 (Cint (high_s ofs)) ::
+              mk1 (Cint (low_s ofs)) temp :: k
+          else
+             addimm temp GPR1 ofs (mk1 (Cint Int.zero) temp :: k))
   | _, _ =>
       Error(msg "Asmgen.transl_memory_access")
   end.
@@ -779,28 +805,28 @@ Definition transl_load (chunk: memory_chunk) (addr: addressing)
   match chunk with
   | Mint8signed =>
       do r <- ireg_of dst;
-      transl_memory_access (Plbz r) (Plbzx r) addr args GPR12 (Pextsb r r :: k)
+      transl_memory_access (Plbz r) (Plbzx r) true addr args GPR12 (Pextsb r r :: k)
   | Mint8unsigned =>
       do r <- ireg_of dst;
-      transl_memory_access (Plbz r) (Plbzx r) addr args GPR12 k
+      transl_memory_access (Plbz r) (Plbzx r) true addr args GPR12 k
   | Mint16signed =>
       do r <- ireg_of dst;
-      transl_memory_access (Plha r) (Plhax r) addr args GPR12 k
+      transl_memory_access (Plha r) (Plhax r) true addr args GPR12 k
   | Mint16unsigned =>
       do r <- ireg_of dst;
-      transl_memory_access (Plhz r) (Plhzx r) addr args GPR12 k
+      transl_memory_access (Plhz r) (Plhzx r) true addr args GPR12 k
   | Mint32 =>
       do r <- ireg_of dst;
-      transl_memory_access (Plwz r) (Plwzx r) addr args GPR12 k
+      transl_memory_access (Plwz r) (Plwzx r) true addr args GPR12 k
   | Mint64 =>
       do r <- ireg_of dst;
-      transl_memory_access (Pld r) (Pldx r) addr args GPR12 k
+      transl_memory_access (Pld r) (Pldx r) false addr args GPR12 k
   | Mfloat32 =>
       do r <- freg_of dst;
-      transl_memory_access (Plfs r) (Plfsx r) addr args GPR12 k
+      transl_memory_access (Plfs r) (Plfsx r) true addr args GPR12 k
   | Mfloat64 =>
       do r <- freg_of dst;
-      transl_memory_access (Plfd r) (Plfdx r) addr args GPR12 k
+      transl_memory_access (Plfd r) (Plfdx r) true addr args GPR12 k
   | _ =>
       Error (msg "Asmgen.transl_load")
   end.
@@ -811,22 +837,22 @@ Definition transl_store (chunk: memory_chunk) (addr: addressing)
   match chunk with
   | Mint8signed | Mint8unsigned =>
       do r <- ireg_of src;
-      transl_memory_access (Pstb r) (Pstbx r) addr args temp k
+      transl_memory_access (Pstb r) (Pstbx r) true addr args temp k
   | Mint16signed | Mint16unsigned =>
       do r <- ireg_of src;
-      transl_memory_access (Psth r) (Psthx r) addr args temp k
+      transl_memory_access (Psth r) (Psthx r) true addr args temp k
   | Mint32  =>
       do r <- ireg_of src;
-      transl_memory_access (Pstw r) (Pstwx r) addr args temp k
+      transl_memory_access (Pstw r) (Pstwx r) true addr args temp k
   | Mint64  =>
       do r <- ireg_of src;
-      transl_memory_access (Pstd r) (Pstdx r) addr args temp k
+      transl_memory_access (Pstd r) (Pstdx r) false addr args temp k
   | Mfloat32 =>
       do r <- freg_of src;
-      transl_memory_access (Pstfs r) (Pstfsx r) addr args temp k
+      transl_memory_access (Pstfs r) (Pstfsx r) true addr args temp k
   | Mfloat64 =>
       do r <- freg_of src;
-      transl_memory_access (Pstfd r) (Pstfdx r) addr args temp k
+      transl_memory_access (Pstfd r) (Pstfdx r) true addr args temp k
   | _ =>
       Error (msg "Asmgen.transl_store")
   end.
